Use sets of states for RTS continuations

common/ModuleSemantics.v
@@ -79,61 +79,38 @@ End FComp.
 
 (** To go from the flat composition to horizontal composition, we
   introduce the following resolution operator. [Res] eliminates
-  external calls to internal functions by replacing them with a nested
-  execution of the transition system. Each [Res.state] is a stack of
-  states of [L]: normal execution operates on the topmost state;
-  a recursive call into [L] pushes the nested initial state on the
-  stack; reaching a final state causes the topmost state to be popped
-  and the caller to be resumed, or returns to the environment when
-  we reach the last one. *)
+  external calls to internal functions by using the corresponding
+  query to immediately reenter the component. Note that this operator
+  is only well-behaved for deterministic transition systems: in a
+  nondeterministic transition system, a switching final state may
+  coexist with other steps. If the switch results in a query that goes
+  initially wrong, this behavior would be cancelled out by the
+  alternative step. *)
 
 Module Res.
   Section RESOLVE.
     Context {li} (sw: reply li -> query li) (L: Smallstep.semantics li).
 
-    (** When switching occurs, we use an intermediate [resumed] state
-      before starting up again. This is important for two reasons.
-      First, in a nondeterministic transition system, a switching
-      final state may coexist with other steps. If the switch results
-      in a query that goes initially wrong, this behavior would be
-      cancelled out by the alternative step, whereas the approach
-      below allows us to first transition to the [resumed] step, then
-      go wrong. Second, the strategy-level horizontal composition will
-      also have such a step, introduced as the initial step of the
-      embedding for the component being switched to, so that using the
-      extra step allows the commutation proof between horizontal
-      composition and embedding to be a simple lockstep simulation. *)
-
-    Inductive state {A} :=
-      | running (s : A)
-      | resumed (S : A -> Prop).
-
-    Inductive step ge : state -> trace -> state -> Prop :=
+    Inductive step ge : state L -> trace -> state L -> Prop :=
       | step_internal s t s':
           Smallstep.step L ge s t s' ->
-          step ge (running s) t (running s')
-      | step_switch s r k S:
+          step ge s t s'
+      | step_switch s r k s':
           Smallstep.final_state L s r k ->
-          k (sw r) = Some S ->
-          step ge (running s) E0 (resumed S)
-      | step_resume (S: Smallstep.state L -> Prop) s :
-          S s ->
-          step ge (resumed S) E0 (running s).
+          resume k (sw r) s' ->
+          step ge s E0 s'.
 
-    Definition liftk {A} (k: cont li A) : cont li state :=
-      fun q => option_map (set_map running) (k q).
-
-    Inductive final_state : state -> reply li -> _ -> Prop :=
+    Inductive final_state : state L -> reply li -> _ -> Prop :=
       final_state_intro s r k :
         Smallstep.final_state L s r k ->
         k (sw r) = None ->
-        final_state (running s) r (liftk k).
+        final_state s r k.
 
     Definition semantics: Smallstep.semantics li :=
       {|
-        Smallstep.state := state;
+        Smallstep.state := state L;
         Smallstep.step := step;
-        Smallstep.initial_state := liftk (initial_state L);
+        Smallstep.initial_state := initial_state L;
         Smallstep.final_state := final_state;
         Smallstep.globalenv := globalenv L;
         Smallstep.symbolenv := symbolenv L;
