games/GameSemantics.v
@@ -28,7 +28,7 @@ Record modsem {li : language_interface} :=
   {
     modsem_state : Type;
     modsem_lts :> rts li modsem_state;
-    modsem_entry : input li -> option modsem_state;
+    modsem_entry : input li -> option (modsem_state -> Prop);
   }.
 
 Arguments modsem : clear implicits.
@@ -39,8 +39,8 @@ Record modref {li} (α β : modsem li) : Prop :=
       rel (modsem_state α) (modsem_state β);
     modref_sim :
       RTS.sim modref_state (modsem_lts α) (modsem_lts β);
-    modref_init :
-      forall q, option_rel modref_state (modsem_entry α q) (modsem_entry β q);
+    modref_init q :
+      option_rel (set_le modref_state) (modsem_entry α q) (modsem_entry β q);
   }.
 
 
@@ -53,19 +53,19 @@ Module Behavior.
     (** ** Transition system *)
 
     Inductive state {A} :=
-      | resumed (k : A -> Prop)
-      | running (s : A).
+      | running (s : A)
+      | wrong.
 
-    Definition liftk {A} (k : cont li A) (q : input li): option state :=
-      option_map resumed (k q).
+    Inductive lifts {A} (S : A -> Prop) : state -> Prop :=
+      | lifts_goes_wrong : ~ ex S -> lifts S wrong
+      | lifts_resumes s : S s -> lifts S (running s).
+
+    Definition liftk {A} (k : cont li A): cont li state :=
+      fun q => option_map lifts (k q).
 
     Inductive step : rts li state :=
-      | step_resumed (k : Smallstep.state L -> Prop) s :
-          k s ->
-          step (resumed k) (RTS.internal (running s))
-      | step_goes_initially_wrong (k : Smallstep.state L -> Prop) :
-          ~ ex k ->
-          step (resumed k) (RTS.goes_wrong)
+      | step_goes_initially_wrong :
+          step wrong (RTS.goes_wrong)
       | step_internal s s' :
           Step L s E0 s' ->
           step (running s) (RTS.internal (running s'))
@@ -75,7 +75,7 @@ Module Behavior.
       | step_goes_wrong s :
           Nostep L s ->
           (forall r k, ~ final_state L s r k) ->
-          step (running s) (RTS.goes_wrong).
+          step (running s) (RTS.internal wrong).
 
     Definition of : modsem li :=
       {|
@@ -83,8 +83,6 @@ Module Behavior.
         modsem_lts := RTS.obs step;
         modsem_entry := liftk (initial_state L);
       |}.
-
-    (** ** Properties *)
 
     (** The following properties of the transition system will be
       useful in the soundness proof below. *)
@@ -110,66 +108,41 @@ Module Behavior.
 
     Definition safe S :=
       match S with
-        | resumed k => ex k /\ forall s, k s -> Smallstep.safe L s
         | running s => Smallstep.safe L s
+        | wrong => False
       end.
 
     Lemma unsafe_goes_wrong S:
       ~ safe S ->
       RTS.obs step S RTS.goes_wrong.
     Proof.
-      assert (forall s, ~ Smallstep.safe L s ->
-                        RTS.obs step (running s) RTS.goes_wrong).
-      {
-        intros s HS.
-        apply not_all_ex_not in HS as [s' HS].
-        apply not_all_ex_not in HS as [Hs' HS].
-        revert HS. pattern s, s'. revert s s' Hs'.
-        eapply star_E0_ind; eauto; intros.
+      intros HS.
+      destruct S as [ | ]; simpl in *; eauto using step_goes_initially_wrong.
+      apply not_all_ex_not in HS as [s' HS].
+      apply not_all_ex_not in HS as [Hs' HS].
+      revert HS. pattern s, s'. revert s s' Hs'.
+      eapply star_E0_ind; eauto; intros.
+      - apply RTS.obs_external with wrong; auto.
+        + constructor.
         + econstructor; eauto.
           eapply step_goes_wrong; firstorder.
-        + eapply RTS.obs_internal; eauto.
-          constructor; eauto.
-      }
-      intros HS.
-      destruct S as [ | ]; simpl in *; eauto.
-      apply not_and_or in HS as [HS | HS].
-      - econstructor; eauto.
-        constructor; eauto.
-      - eapply not_all_ex_not in HS as [s HS].
-        eapply not_all_ex_not in HS as [Hs HS].
-        eapply RTS.obs_internal; eauto.
+      - eapply RTS.obs_internal; eauto.
         constructor; eauto.
     Qed.
 
     (** ** Determinism *)
 
     (** From deterministic small-step semantics, we can obtain a
-      deterministic transition system.
-      However we need to restrict the state space in order to avoid
-      non-deterministic continuations. *)
-
-    Definition state_determ (s : state (A := Smallstep.state L)) : Prop :=
-      match s with
-        | resumed k => forall s1 s2, k s1 -> k s2 -> s1 = s2
-        | _ => True
-      end.
-
-    Definition step_determ : rts li (sig state_determ) :=
-      fun s r =>
-        step (proj1_sig s) (RTS.behavior_map (@proj1_sig _ _) r).
+      deterministic transition system. *)
 
     Lemma program_lts_determ:
       Smallstep.determinate L ->
-      RTS.deterministic step_determ.
+      RTS.deterministic step.
     Proof.
-      intros HL [s Hs] r1 r2 H1 H2.
-      red in H1, H2. simpl in *.
-      destruct r1 as [[s' Hs'] | m k1 | | ]; inversion H1; clear H1; subst.
+      intros HL s r1 r2 H1 H2.
     Abort. (* determinism -- tedious but straightforward *)
 
   End LTS.
-
 
   (** ** Monotonicity *)
 
@@ -180,14 +153,12 @@ Module Behavior.
 
     We use the following alternating simulation relation. *)
 
-  Inductive state_rel {A B} (R : rel A B) : rel state state :=
-    | resumed_rel (k1 k2 : _ -> Prop) :
-        (forall s2, k2 s2 -> exists s1, k1 s1) ->
-        (forall s1 s2, k1 s1 -> k2 s2 -> exists s2', k2 s2' /\ R s1 s2') ->
-        state_rel R (resumed k1) (resumed k2)
+  Inductive state_rel {A B} R : rel (@state A) (@state B) :=
     | running_rel s1 s2 :
         R s1 s2 ->
-        state_rel R (running s1) (running s2).
+        state_rel R (running s1) (running s2)
+    | wrong_rel S1 :
+        state_rel R S1 wrong.
 
   Hint Constructors state_rel.
 
@@ -198,7 +169,8 @@ Module Behavior.
     revert s. cofix IH.
     intros.
     destruct H. inversion H; clear H; subst.
-    econstructor; eauto.
+    - econstructor; eauto.
+    - destruct H0. inversion H.
   Qed.
 
   Lemma forever_silent_rts {li} (L : semantics li) s:
@@ -226,18 +198,52 @@ Module Behavior.
 
   Hint Extern 10 => rstep : coqrel.
 
+  Lemma bsim_lifts {A B} (R : rel A B) (k1 k2 : _ -> Prop) :
+    (forall s, k2 s -> ex k1) ->
+    (forall s, k2 s -> set_le R k1 k2) ->
+    set_le (state_rel R) (lifts k1) (lifts k2).
+  Proof.
+    intros Hex Hk s1 Hs1.
+    destruct Hs1 as [Hk1 | s1 Hs1].
+    - exists wrong; split; constructor.
+      intros [s2 Hs2]. eauto.
+    - destruct (classic (ex k2)) as [[s2e Hs2e] | H2].
+      + edestruct Hk as (s2 & Hs2 & Hs); eauto.
+        exists (running s2); split; constructor; eauto.
+      + exists wrong; split; constructor; eauto.
+  Qed.
+
   Lemma bsim_sound_liftk {li} L1 L2 ind ord ms (k1 k2: cont li _) q :
     @bsim_properties li L2 L1 ind ord ms ->
     bsim_match_cont (rel_ex ms) k2 k1 ->
-    option_rel (state_rel (flip (rel_ex ms))) (liftk k1 q) (liftk k2 q).
+    option_rel (set_le (state_rel (flip (rel_ex ms)))) (liftk k1 q) (liftk k2 q).
   Proof.
     intros HL Hk. unfold liftk.
-    specialize (Hk q). destruct Hk as [S1 S2 HS | ]; constructor.
-    constructor.
+    specialize (Hk q). destruct Hk as [S2 S1 HS | ]; constructor.
+    eapply bsim_lifts.
     - intros.
       edestruct @bsim_sets_exists as (? & ? & ?); eauto.
-    - intros. unfold flip, rel_ex.
+    - intros s1 Hs1 s2 Hs2. unfold flip, rel_ex.
       edestruct @bsim_sets_match as (? & ? & ?); eauto.
+  Qed.
+
+  Lemma reachable_inv {li} (L : semantics li) s S':
+    Smallstep.safe L s ->
+    RTS.reachable (step L) (running s) S' ->
+    exists s', S' = running s' /\ Star L s E0 s'.
+  Proof.
+    intros Hs HS'.
+    change (safe L (running s)) in Hs.
+    remember (running s) as S eqn:HS. revert s HS.
+    induction HS' as [S | S1 S2 S3 HS12 HS23].
+    - eauto using star_refl.
+    - inversion HS12; clear HS12; subst.
+      + inversion 1; clear HS; subst.
+        edestruct IHHS23 as (s'' & Hs'' & Hsteps); eauto using star_step.
+        simpl in Hs |- *. eauto using star_safe, star_one.
+      + edestruct Hs as [(r & k & Hk) | (t & s' & Hs')]; eauto using star_refl.
+        * eelim H2; eauto.
+        * eelim H0; eauto.
   Qed.
 
   Lemma bsim_sound_step {li} (L1 L2: semantics li) ind ord ms:
@@ -247,74 +253,50 @@ Module Behavior.
       (RTS.obs (step L2)).
   Proof.
     set (R := flip (rel_ex ms)). unfold flip, rel_ex in R.
-    intros HL S1 S2 HS S1' HS1'.
+    intros HL S1 S2 HS r1 Hr1.
     destruct (classic (safe L2 S2)) as [HS2 | ];
       [ | now eauto using unsafe_goes_wrong with coqrel ].
-    destruct HS1' as [HS1 | S1' r Hrext Hr HS1'].
+    destruct HS as [s1 s2 Hs | ]; simpl in HS2; try contradiction.
+    inversion Hr1 as [Hs1 | S1 r Hrext Hr Hs1']; clear Hr1; subst.
 
     - (* Divergence *)
       exists RTS.diverges. split; [ | rauto].
-      destruct HS.
-      + destruct HS1 as [S1' HS1' HS1].
-        inversion HS1'; clear HS1'; subst.
-        simpl in HS2. destruct HS2 as [[s2 Hks2] Hk].
-        edestruct H0 as (s2' & Hs2' & i & Hs'); eauto.
-        apply RTS.obs_diverges.
-        econstructor.
-        * econstructor; eauto.
-        * eapply forever_internal_bsim; eauto.
-      + destruct H as [i H].
-        apply RTS.obs_diverges.
-        eapply forever_internal_bsim; eauto.
+      destruct Hs as [i Hs].
+      apply RTS.obs_diverges.
+      eapply forever_internal_bsim; eauto.
 
     - (* Observation *)
-      revert S2 HS HS2.
-      induction HS1'; intros.
+      assert (HS1: Smallstep.safe L1 s1) by (destruct Hs; eauto using bsim_safe).
+      apply reachable_inv in Hs1' as (s1' & ? & Hs1'); auto; subst.
+      revert s2 Hs HS2. clear HS1.
+      revert Hr. pattern s1, s1'. revert s1 s1' Hs1'.
+      apply star_E0_ind.
 
-      + (* Noisy steps *)
-        destruct Hr; inversion HS; clear HS; inversion Hrext; clear Hrext; subst.
-        * (* Can't initially go wrong *)
-          simpl in HS2. destruct HS2 as [[s2 Hs2] Hk2].
-          edestruct H1 as [s1 Hs1]; eauto.
-          elim H; eauto.
-        * (* Final states *)
-          destruct H1 as (i & Hs).
-          eapply bsim_match_final_states in H; eauto.
-          destruct H as (s2' & k2 & Hs2' & Hsk2 & Hk); eauto.
-          exists (RTS.interacts (G:=li) r (liftk k2)). split.
-          -- eapply RTS.obs_external with (running s2'); eauto.
-             ++ constructor; eauto.
-             ++ eapply star_reachable; eauto.
-          -- constructor. intro q.
-             eapply bsim_sound_liftk; eauto.
-        * (* Can't go wrong *)
-          simpl in HS2. subst R. destruct H2 as [i Hs].
-          eapply bsim_safe in HS2; eauto. red in HS2. clear - HS2 H0 H. exfalso.
-          edestruct HS2 as [(r & k & Hs)|(t & s' & Hs')]; eauto using star_refl.
-          -- eapply H0; eauto.
-          -- eapply H; eauto.
+      + (* Final states *)
+        intros s1 Hr s2 Hs Hs2.
+        inversion Hr; clear Hr; subst; try now inversion Hrext.
+        destruct Hs as (i & Hs).
+        eapply bsim_match_final_states in H0; eauto.
+        destruct H0 as (s2' & k2 & Hs2' & Hsk2 & Hk); eauto.
+        exists (RTS.interacts (G:=li) r (liftk k2)). split.
+        * eapply RTS.obs_external with (running s2'); eauto.
+          -- constructor; eauto.
+          -- eapply star_reachable; eauto.
+        * constructor. intro q.
+           eapply bsim_sound_liftk; eauto.
 
       + (* Silent steps *)
-        specialize (IHHS1' Hr). clear Hr a'' HS1'.
-        destruct HS; inversion H; clear H; subst.
-        * (* Resumed execution *)
-          simpl in HS2. destruct HS2 as [[s2 Hs2] Hk2].
-          edestruct H1 as (s2' & Hs2' & Hs); eauto.
-          edestruct IHHS1' as (r2 & Hr2 & Hr12); eauto.
-          -- simpl. eauto.
-          -- exists r2. split; eauto.
-             eapply RTS.obs_internal; eauto.
-             constructor; eauto.
-        * (* E0 step *)
-          destruct H0 as [i Hs12]. simpl in HS2.
-          edestruct (bsim_E0_star HL) as (j & s2' & Hs2' & Hs12');
-            eauto using star_one.
-          edestruct IHHS1' as (r2 & Hr2 & Hr12).
-          -- constructor. eexists. eauto.
-          -- simpl. eauto using star_safe.
-          -- exists r2. split; eauto.
-             eapply RTS.obs_reachable; eauto.
-             eapply star_reachable; eauto.
+        intros s1 s1' s1'' Hs1' Hs1'' Hr1 s2 Hs Hs2.
+        specialize (Hs1'' Hr1). clear Hr1 s1''.
+        destruct Hs as [i Hs].
+        edestruct (bsim_E0_star HL) as (j & s2' & Hs2' & Hs12');
+          eauto using star_one.
+        edestruct Hs1'' as (r2 & Hr2 & Hr12).
+        -- eexists. eauto.
+        -- eauto using star_safe.
+        -- exists r2. split; eauto.
+           eapply RTS.obs_reachable; eauto.
+           eapply star_reachable; eauto.
   Qed.
 
   Global Instance bsim_sound:
